src/Lib.v
@@ -1,12 +1,13 @@
-Require Export Hask.Prelude.
 Require Export Hask.Ltac.
 Require Export Hask.Control.Lens.
 Require Export Hask.Control.Monad.
-Require Export Hask.Data.IntMap.
-Require Export Hask.Data.IntSet.
-Require Export Hask.Data.List.
-Require Export Hask.Data.NonEmpty.
-Require Export Hask.Data.Vector.
+Require Export LinearScan.IntMap.
+Require Export LinearScan.IntSet.
+Require Export LinearScan.ListSsr.
+Require Export LinearScan.NonEmpty.
+Require Export LinearScan.Vector.
+Require Export LinearScan.Tactics.
+Require Export Hask.Ssr.
 
 Require Export Coq.Program.Wf.
 Require Export Coq.Sorting.Sorted.
@@ -30,3 +31,9 @@ Extraction Implicit widen_fst [ n ].
 
 Extract Inlined Constant widen_id  => "".
 Extract Inlined Constant widen_fst => "Prelude.id".
+
+Definition lebf {a : Type} (f : a -> nat) (n m : a) := f n <= f m.
+
+Definition flip `(f : a -> b -> c) : b -> a -> c := fun y x => f x y.
+
+Notation "f $ x" := (f x) (at level 60, right associativity, only parsing).
