src/IntMap.v
@@ -1,0 +1,194 @@
+Require Import Hask.Ssr.
+Require Import LinearScan.ListSsr.
+Require Import LinearScan.NonEmpty.
+
+Set Implicit Arguments.
+Unset Strict Implicit.
+Unset Printing Implicit Defensive.
+Generalizable All Variables.
+
+Inductive IntMap (a : Type) := getIntMap of seq (nat * a).
+
+Arguments getIntMap {a} _.
+
+Definition emptyIntMap {a} := @getIntMap a [::].
+
+Definition IntMap_fromList {a} := @getIntMap a.
+
+Definition IntMap_size : forall a, IntMap a -> nat :=
+  fun _ m => let: getIntMap x := m in size x.
+
+(* We needn't bother defining these in Coq, since they only matter to the
+   extracted Haskell code, and there we use the definitions from
+   [Data.IntMap]. *)
+Definition IntMap_lookup : forall a, nat -> IntMap a -> option a :=
+  fun _ k m => let: getIntMap x := m in maybeLookup x k.
+
+Definition IntMap_member : forall a, nat -> IntMap a -> bool :=
+  fun _ k m => if IntMap_lookup k m is Some _ then true else false.
+
+Notation "f $ x" := (f x) (at level 60, right associativity, only parsing).
+
+Definition IntMap_alter : forall a,
+  (option a -> option a) -> nat -> IntMap a -> IntMap a :=
+  fun _ f k m =>
+    let: getIntMap xs := m in @getIntMap _ $
+    if IntMap_lookup k m is Some x
+    then
+      foldr (fun z acc =>
+               let: (a, b) := z in
+               if a == k
+               then if f (Some x) is Some x'
+                    then rcons acc (k, x')
+                    else acc
+               else z :: acc)
+            [::] xs
+    else if f None is Some x
+         then rcons xs (k, x)
+         else xs.
+
+Definition IntMap_insert : forall a, nat -> a -> IntMap a -> IntMap a :=
+  fun _ k x m => IntMap_alter (fun _ => Some x) k m.
+
+Definition IntMap_map {a b} (f : a -> b) (m : IntMap a) : IntMap b :=
+  let: getIntMap xs := m in
+  getIntMap (map (fun x => (fst x, f (snd x))) xs).
+
+Lemma IntMap_map_id : forall a (m : IntMap a), IntMap_map id m = m.
+Proof.
+  move=> a [m].
+  case: m => //= [m l].
+  case: m => /= ? ?.
+  congr (getIntMap ((_, _) :: _)).
+  elim: l => [|x xs IHl] //=.
+  rewrite IHl.
+  by case: x.
+Qed.
+
+Lemma IntMap_map_comp : forall a b c (m : IntMap a) (f : b -> c) (g : a -> b),
+  IntMap_map f \o IntMap_map g =1 IntMap_map (f \o g).
+Proof.
+  move=> a b c [m] f g [xs] /=.
+  elim: xs => //= [? ? IHxs].
+  rewrite -map_comp /funcomp in IHxs *.
+  by congr (getIntMap _).
+Qed.
+
+Definition IntMap_mapWithKey {a b} (f : nat -> a -> b) (m : IntMap a) :
+  IntMap b :=
+  let: getIntMap xs := m in
+  let f z := let: (k, x) := z in (k, f k x) in
+  getIntMap (map f xs).
+
+Lemma getIntMap_inj {a} : injective (@getIntMap a).
+Proof. by move=> ? ?; invert. Qed.
+
+Lemma IntMap_mapWithKey_id : forall a (m : IntMap a),
+  IntMap_mapWithKey (const id) m = m.
+Proof.
+  move=> a [m].
+  elim: m => //= [[x y] ? ?].
+  congr (getIntMap ((x, y) :: _)).
+  exact: getIntMap_inj.
+Qed.
+
+Lemma IntMap_mapWithKey_comp :
+  forall a b c (m : IntMap a) (f : b -> c) (g : a -> b),
+    IntMap_mapWithKey (const f) \o IntMap_mapWithKey (const g)
+      =1 IntMap_mapWithKey (const (f \o g)).
+Proof.
+  move=> a b c [m] f g [xs] /=.
+  elim: xs => //= [[x y] xs IHxs].
+  congr (getIntMap (_ :: _)).
+  exact: getIntMap_inj.
+Qed.
+
+(* The implementation of this function is in LinearScan.Utils.hs *)
+Definition IntMap_mergeWithKey' {a b c}
+  (combine : nat -> a -> b -> option c)
+  (only1 : seq (nat * a) -> seq (nat * c))
+  (only2 : seq (nat * b) -> seq (nat * c))
+  (m1 : seq (nat * a)) (m2 : seq (nat * b)) : seq (nat * c) := [::].
+
+Definition IntMap_mergeWithKey {a b c} (combine : nat -> a -> b -> option c)
+  (only1 : IntMap a -> IntMap c) (only2 : IntMap b -> IntMap c)
+  (m1 : IntMap a) (m2 : IntMap b) : IntMap c :=
+  let: getIntMap xs1 := m1 in
+  let: getIntMap xs2 := m2 in
+  let only1' xs :=
+    let: getIntMap xs' := only1 (getIntMap xs) in xs' in
+  let only2' xs :=
+    let: getIntMap xs' := only2 (getIntMap xs) in xs' in
+  getIntMap (IntMap_mergeWithKey' combine only1' only2' xs1 xs2).
+
+Definition IntMap_foldl {a b} (f : a -> b -> a) (z : a) (m : IntMap b) : a :=
+  let: getIntMap xs := m in foldl (fun acc x => f acc (snd x)) z xs.
+
+Definition IntMap_foldr {a b} (f : b -> a -> a) (z : a) (m : IntMap b) : a :=
+  let: getIntMap xs := m in foldr (fun x => f (snd x)) z xs.
+
+Definition IntMap_foldlWithKey
+  {a b} (f : a -> nat -> b -> a) (z : a) (m : IntMap b) : a :=
+  let: getIntMap xs := m in foldl (fun acc x => f acc (fst x) (snd x)) z xs.
+
+Definition IntMap_foldrWithKey
+  {a b} (f : b -> nat -> a -> a) (z : a) (m : IntMap b) : a :=
+  let: getIntMap xs := m in foldr (fun x => f (snd x) (fst x)) z xs.
+
+Definition IntMap_toList {a} (m : IntMap a) : seq (nat * a) :=
+  let: getIntMap xs := m in xs.
+
+Definition IntMap_addToList (k : nat) `(x : a) (m : IntMap (seq a)) :
+  IntMap (seq a) :=
+  IntMap_alter (fun mxs => Some (if mxs is Some xs
+                                 then x :: xs
+                                 else [:: x])) k m.
+
+Definition IntMap_combine {a b c}
+  (f : nat -> option a -> option b -> option c) :
+  IntMap a -> IntMap b -> IntMap c :=
+  IntMap_mergeWithKey
+    (fun idx x y => f idx (Some x) (Some y))
+    (IntMap_foldrWithKey
+       (fun x idx rest =>
+          let mres := f idx (Some x) None in
+          if mres is Some res
+          then IntMap_insert idx res rest
+          else rest) emptyIntMap)
+    (IntMap_foldrWithKey
+       (fun y idx rest =>
+          let mres := f idx None (Some y) in
+          if mres is Some res
+          then IntMap_insert idx res rest
+          else rest) emptyIntMap).
+
+Section EqIntMap.
+
+Variable a : eqType.
+
+Definition eqIntMap (s1 s2 : IntMap a) :=
+  match s1, s2 with
+  | getIntMap xs, getIntMap ys => xs == ys
+  end.
+
+Lemma eqIntMapP : Equality.axiom eqIntMap.
+Proof.
+  move.
+  case=> [s1].
+  case=> [s2] /=.
+  case: (s1 =P s2) => [<-|neqx]; last by right; case.
+  by constructor.
+Qed.
+
+Canonical IntMap_eqMixin := EqMixin eqIntMapP.
+Canonical IntMap_eqType := Eval hnf in EqType (IntMap a) IntMap_eqMixin.
+
+End EqIntMap.
+
+Definition IntMap_groupOn {a} (p : a -> nat) (l : seq a) :
+  IntMap (NonEmpty a) :=
+  forFold emptyIntMap l $ fun acc x =>
+    let n := p x in
+    IntMap_alter (fun mxs => if mxs is Some xs
+                             then Some (NE_Cons x xs)
+                             else Some [::: x]) n acc.
