src/Verify.v
@@ -1,11 +1,12 @@
 Require Import LinearScan.Lib.
-Require Import Hask.Control.Monad.Trans.State.
 Require Import LinearScan.UsePos.
 Require Import LinearScan.Interval.
 Require Import LinearScan.Blocks.
 Require Import LinearScan.Resolve.
 Require Import LinearScan.Allocate.
 Require Import LinearScan.Loops.
+Require Import Hask.Control.Monad.Trans.State.
+Require Import Hask.Control.Monad.
 
 Set Implicit Arguments.
 Unset Strict Implicit.
@@ -217,7 +218,7 @@ Variable intervals : seq (Allocation maxReg).
 Variable useVerifier : UseVerifier.
 
 Definition errorsT (errs : seq AllocError) : Verified unit :=
-  st <-- use _verDesc ;;
+  st <- use _verDesc ;
   _verErrors %= fun m =>
     flip (IntMap_insert pc) m $
       if IntMap_lookup pc m is Some (d, prevErrs)
@@ -237,7 +238,7 @@ Definition allocationsAt (pos : nat) : seq (Allocation maxReg) :=
            ibeg int <= pos < iend int].
 
 Definition allocationFor (var : VarId) (pos : nat) : option (option PhysReg) :=
-  match [seq i <- allocationsAt pos | ivar (intVal i) == var] with
+  match filter (fun i => ivar (intVal i) == var) (allocationsAt pos) with
   | [::]   => None                (* not allocated here *)
   | [:: a] => Some (intReg a)     (* allocated in reg or on stack *)
   | _      => None                (* over-allocated! but see the Theorem
@@ -257,76 +258,76 @@ Definition checkAllocation
 
 Definition reserveReg (reg : PhysReg) (var : VarId) :
   Verified unit :=
-  addMove $ RSAllocReg var reg ;;
-  st <-- use _verDesc ;;
-  if prop (vnth (rsAllocs st) reg ^_ reservation == None) is Some H
-  then _verState .= packRegState (ReserveRegS var H)
-  else if vnth (rsAllocs st) reg ^_ reservation is Some v
-       then when (v != var) $
-              errorT $ RegAlreadyReservedToVar reg v var
-       else pure tt.
+  addMove (RSAllocReg var reg) ;;
+  (st <- use _verDesc ;
+   if prop (vnth (rsAllocs st) reg ^_ reservation == None) is Some H
+   then _verState .= packRegState (ReserveRegS var H)
+   else if vnth (rsAllocs st) reg ^_ reservation is Some v
+        then when (v != var) $
+               errorT $ RegAlreadyReservedToVar reg v var
+        else pure tt).
 
 Definition isReserved (reg : PhysReg) : Verified (option VarId) :=
-  st <-- use _verDesc ;;
+  st <- use _verDesc ;
   pure (vnth (rsAllocs st) reg ^_ reservation).
 
 Definition checkReservation (reg : PhysReg) (var : VarId) : Verified unit :=
-  st <-- use _verDesc ;;
+  st <- use _verDesc ;
   let err := errorT $ VarNotReservedForReg var reg
                         (vnth (rsAllocs st) reg ^_ reservation) 1 in
-  res <-- isReserved reg ;;
+  res <- isReserved reg ;
   if res is Some var'
   then unless (var == var') err
   else err.
 
 Definition releaseReg (reg : PhysReg) (var : VarId) :
   Verified unit :=
-  addMove $ RSFreeReg reg var ;;
-  st <-- use _verDesc ;;
-  if prop (vnth (rsAllocs st) reg ^_ reservation == Some var) is Some H
-  then _verState .= packRegState (ReleaseRegS H)
-  else errorT $ VarNotReservedForReg var reg
-                  (vnth (rsAllocs st) reg ^_ reservation) 2.
+  addMove (RSFreeReg reg var) ;;
+  (st <- use _verDesc ;
+   if prop (vnth (rsAllocs st) reg ^_ reservation == Some var) is Some H
+   then _verState .= packRegState (ReleaseRegS H)
+   else errorT $ VarNotReservedForReg var reg
+                   (vnth (rsAllocs st) reg ^_ reservation) 2).
 
 Definition clearReg (reg : PhysReg) (var : VarId) : Verified unit :=
-  addMove $ RSClearReg reg var ;;
-  st <-- use _verDesc ;;
-  if prop (vnth (rsAllocs st) reg ^_ residency == Some var) is Some H
-  then _verState .= packRegState (ClearRegS H)
-  else let err := errorT $ VarNotResidentForReg var reg
-                             (vnth (rsAllocs st) reg ^_ residency) 2 in
-       if useVerifier is VerifyEnabledStrict
-       then err
-       else if vnth (rsAllocs st) reg ^_ residency is None
-            then pure tt
-            else err.
+  addMove (RSClearReg reg var) ;;
+  (st <- use _verDesc ;
+   if prop (vnth (rsAllocs st) reg ^_ residency == Some var) is Some H
+   then _verState .= packRegState (ClearRegS H)
+   else let err := errorT $ VarNotResidentForReg var reg
+                              (vnth (rsAllocs st) reg ^_ residency) 2 in
+        if useVerifier is VerifyEnabledStrict
+        then err
+        else if vnth (rsAllocs st) reg ^_ residency is None
+             then pure tt
+             else err).
 
 Definition assignReg (reg : PhysReg) (var : VarId) : Verified unit :=
-  addMove $ RSAssignReg var reg ;;
-  st <-- use _verDesc ;;
-  if prop (vnth (rsAllocs st) reg ^_ reservation == Some var) is Some H
-  then (* When a variable is assigned to a register, all of its older
-          values in other registers are invalidated. *)
-       vfoldr_with_index (fun reg x act =>
-                            if fst x == Some var
-                            then clearReg reg var >> act
-                            else act) (pure tt) (rsAllocs st) ;;
-       _verState .= packRegState (AssignRegS H)
-  else let err := errorT $ VarNotReservedForReg var reg
-                         (vnth (rsAllocs st) reg ^_ reservation) 3 in
-       if useVerifier is VerifyEnabledStrict
-       then err
-       else if vnth (rsAllocs st) reg ^_ reservation is None
-            then pure tt
-            else err.
+  addMove (RSAssignReg var reg) ;;
+  (st <- use _verDesc ;
+   if prop (vnth (rsAllocs st) reg ^_ reservation == Some var) is Some H
+   then (* When a variable is assigned to a register, all of its older
+           values in other registers are invalidated. *)
+        vfoldr_with_index (fun reg x act =>
+                             if fst x == Some var
+                             then clearReg reg var >> act
+                             else act) (pure tt) (rsAllocs st) ;;
+        _verState .= packRegState (AssignRegS H)
+   else let err := errorT $ VarNotReservedForReg var reg
+                          (vnth (rsAllocs st) reg ^_ reservation) 3 in
+        if useVerifier is VerifyEnabledStrict
+        then err
+        else if vnth (rsAllocs st) reg ^_ reservation is None
+             then pure tt
+             else err).
 
 Definition isResident (reg : PhysReg) : Verified (option VarId) :=
-  st <-- use _verDesc ;;
+  st <- use _verDesc ;
   pure (vnth (rsAllocs st) reg ^_ residency).
 
 Definition checkResidency (reg : PhysReg) (var : VarId) : Verified unit :=
-  st <-- use _verDesc ;;
-  res <-- isResident reg ;;
+  st  <- use _verDesc ;
+  res <- isResident reg ;
   let err := errorT $ VarNotResidentForReg var reg res 1 in
   if useVerifier is VerifyEnabledStrict
   then if res is Some var'
@@ -335,36 +336,36 @@ Definition checkResidency (reg : PhysReg) (var : VarId) : Verified unit :=
   else pure tt.
 
 Definition isStackAllocated (var : VarId) : Verified bool :=
-  st <-- use _verDesc ;;
+  st <- use _verDesc ;
   pure (IntSet_member var (rsStack st)).
 
 Definition checkStack (var : VarId) : Verified unit :=
-  st  <-- use _verDesc ;;
-  res <-- isStackAllocated var ;;
+  st  <- use _verDesc ;
+  res <- isStackAllocated var ;
   let err := errorT $ StackNotAllocatedForVar var in
   if useVerifier is VerifyEnabledStrict
   then unless res err
   else pure tt.
 
 Definition allocStack (var : VarId) : Verified unit :=
-  addMove $ RSAllocStack var ;;
-  st <-- use _verDesc ;;
-  if prop (~~ IntSet_member var (rsStack st)) is Some H
-  then _verState .= packRegState (AllocStackS H)
-  else let err := errorT $ StackAlreadyAllocatedForVar var in
-       if useVerifier is VerifyEnabledStrict
-       then err
-       else pure tt.
+  addMove (RSAllocStack var) ;;
+  (st <- use _verDesc ;
+   if prop (~~ IntSet_member var (rsStack st)) is Some H
+   then _verState .= packRegState (AllocStackS H)
+   else let err := errorT $ StackAlreadyAllocatedForVar var in
+        if useVerifier is VerifyEnabledStrict
+        then err
+        else pure tt).
 
 Definition freeStack (var : VarId) : Verified unit :=
-  addMove $ RSFreeStack var ;;
-  st <-- use _verDesc ;;
-  if prop (IntSet_member var (rsStack st)) is Some H
-  then _verState .= packRegState (FreeStackS H)
-  else let err := errorT $ StackNotAllocatedForVar var in
-       if useVerifier is VerifyEnabledStrict
-       then err
-       else pure tt.
+  addMove (RSFreeStack var) ;;
+  (st <- use _verDesc ;
+   if prop (IntSet_member var (rsStack st)) is Some H
+   then _verState .= packRegState (FreeStackS H)
+   else let err := errorT $ StackNotAllocatedForVar var in
+        if useVerifier is VerifyEnabledStrict
+        then err
+        else pure tt).
 
 Definition verifyBlockBegin (bid : nat) (liveIns : IntSet) (loops : LoopState) :
   Verified unit :=
@@ -372,7 +373,7 @@ Definition verifyBlockBegin (bid : nat) (liveIns : IntSet) (loops : LoopState) :
   (if IntMap_lookup bid (forwardBranches loops) is Some fwds
    then
      forM_ (IntSet_toList fwds) (fun pred =>
-       exits <-- use _verFinal ;;
+       exits <- use _verFinal ;
        if IntMap_lookup pred exits isn't Some allocs
        then errorT $ UnknownPredecessorBlock bid pred
        else _verState .= allocs)
@@ -382,13 +383,13 @@ Definition verifyBlockBegin (bid : nat) (liveIns : IntSet) (loops : LoopState) :
         when (IntSet_size liveIns > 0) $
           errorT $ BlockWithoutPredecessors bid
      else pure tt)) ;;
-  allocs <-- use _verState ;;
-  _verInit %= IntMap_insert bid allocs.
+  (allocs <- use _verState ;
+   _verInit %= IntMap_insert bid allocs).
 
 Definition verifyBlockEnd (bid : nat) (liveOuts : IntSet) : Verified unit :=
   if useVerifier is VerifyDisabled then pure tt else
   (* Clear out all known allocations, saving them for this block. *)
-  allocs <-- use _verState ;;
+  allocs <- use _verState ;
   _verFinal %= IntMap_insert bid allocs ;;
   _verState .= packRegState StartState.
 
@@ -404,11 +405,12 @@ Definition verifyAllocs (op : opType1)
          make sure that it's not overwriting a variable in a register. *)
 
       when (varKind ref != Input)
-        (st <-- use _verDesc ;;
+        (st <- use _verDesc ;
          if vnth (rsAllocs st) reg ^_ reservation is Some v
          then errorT $ PhysRegAlreadyReservedForVar reg v
          else
-           if [seq i <- allocationsAt pc.-1 | intReg i == Some reg ] is x :: _
+           if filter (fun i => intReg i == Some reg)
+                     (allocationsAt pc.-1) is x :: _
            then errorT $ AllocationDoesNotMatch (ivar (intVal x)) None
                            (Some (option_map (@nat_of_ord maxReg) (intReg x)))
                            pc.-1 0
@@ -437,30 +439,30 @@ Definition verifyResolutions (moves : seq (@ResolvingMove maxReg)) :
   if useVerifier is VerifyDisabled
   then pure moves else
   forFoldM [::] moves $ fun acc mv =>
-    st <-- use _verDesc ;;
+    st <- use _verDesc ;
     match mv with
     | Move fromReg fromVar toReg =>
       checkResidency fromReg fromVar ;;
       checkReservation toReg fromVar ;;
       addMove (weakenResolvingMove mv) ;;
-      pure $ rcons acc mv
+      pure (rcons acc mv)
 
     | Spill fromReg toSpillSlot fromSplit =>
       checkStack toSpillSlot ;;
-      check <-- isResident fromReg ;;
-      (* Spills are not necessary if the variable is not resident. *)
-      if check == Some toSpillSlot
-      then addMove (weakenResolvingMove mv) ;;
-           pure $ rcons acc mv
-      else let mv' := FreeStack maxReg toSpillSlot in
-           addMove (weakenResolvingMove mv') ;;
-           pure $ rcons acc mv'
+      (check <- isResident fromReg ;
+       (* Spills are not necessary if the variable is not resident. *)
+       if check == Some toSpillSlot
+       then addMove (weakenResolvingMove mv) ;;
+            pure (rcons acc mv)
+       else let mv' := FreeStack maxReg toSpillSlot in
+            addMove (weakenResolvingMove mv') ;;
+            pure (rcons acc mv'))
 
     | Restore fromSpillSlot toReg fromSplit =>
       checkStack fromSpillSlot ;;
       checkReservation toReg fromSpillSlot ;;
       addMove (weakenResolvingMove mv) ;;
-      pure $ rcons acc mv
+      pure (rcons acc mv)
 
     | AllocReg toVar toReg    => reserveReg toReg toVar ;; pure acc
     | FreeReg fromReg fromVar => releaseReg fromReg fromVar ;; pure acc
@@ -472,9 +474,9 @@ Definition verifyResolutions (moves : seq (@ResolvingMove maxReg)) :
     | FreeStack fromVar => freeStack fromVar ;; pure acc
 
     | Looped x =>
-      errorT $ LoopInResolvingMoves (weakenResolvingMove x) ;;
+      errorT (LoopInResolvingMoves (weakenResolvingMove x)) ;;
       addMove (weakenResolvingMove mv) ;;
-      pure $ rcons acc mv
+      pure (rcons acc mv)
     end.
 
 Definition verifyTransitions (moves : seq (@ResolvingMove maxReg))
@@ -482,7 +484,7 @@ Definition verifyTransitions (moves : seq (@ResolvingMove maxReg))
   if useVerifier is VerifyDisabled
   then pure tt else
   forM_ moves $ fun mv =>
-    st <-- use _verDesc ;;
+    st <- use _verDesc ;
     match mv with
     | Move fromReg fromVar toReg =>
       checkAllocation (Some (Some fromReg)) fromVar from 4 ;;
@@ -490,9 +492,9 @@ Definition verifyTransitions (moves : seq (@ResolvingMove maxReg))
 
     | Spill fromReg toSpillSlot fromSplit =>
       checkAllocation (Some (Some fromReg)) toSpillSlot from 6 ;;
-      unless fromSplit $ checkAllocation (Some None) toSpillSlot to 7
+      unless fromSplit (checkAllocation (Some None) toSpillSlot to 7)
     | Restore fromSpillSlot toReg fromSplit =>
-      unless fromSplit $ checkAllocation (Some None) fromSpillSlot from 8 ;;
+      unless fromSplit (checkAllocation (Some None) fromSpillSlot from 8) ;;
       checkAllocation (Some (Some toReg)) fromSpillSlot to 9
 
     | AllocReg toVar toReg =>
